src/LCF.Map.fst
@@ -1,0 +1,25 @@
+module LCF.Map
+
+type cmp_on (a:Type0) =
+  a -> a -> bool
+
+type map (a:Type0) (cmp:cmp_on a) (b:Type) =
+  list (a & b)
+
+val map_empty: #a:Type0 -> #cmp:cmp_on a -> #b:Type -> map a cmp b
+let map_empty #a #cmp #b =
+  []
+
+val map_is_empty: #a:Type0 -> #cmp:cmp_on a -> #b:Type -> map a cmp b -> bool
+let map_is_empty #a #cmp #b m =
+  match m with
+  | [] -> true
+  | _ -> false
+
+val map_lookup: #a:Type0 -> #cmp:cmp_on a -> #b:Type -> map a cmp b -> a -> option b
+let map_lookup #a #cmp #b m x0 =
+    List.Tot.fold_right (fun (x, y) acc -> if cmp x x0 then Some y else acc) m None
+
+val map_insert: #a:Type0 -> #cmp:cmp_on a -> #b:Type -> map a cmp b -> a -> b -> map a cmp b
+let map_insert #a #b m x y =
+  (x,y)::m
